demo/Prog.v
@@ -1,0 +1,158 @@
+Require Import Monads ProofMonads List ZArith Program.
+
+Open Scope monad_scope.
+
+Import ListNotations.
+
+Set Implicit Arguments.
+
+Module M := Monads.
+Module PM := ProofMonads.
+
+Section Test.
+
+Definition init_val1 := 0.
+
+Definition init_S1 : nat := init_val1.
+
+Print modify.
+
+Definition add_s (i : nat) : M.State nat unit :=
+  M.modify (fun s => s + i).
+
+Definition minus_s (i : nat) : M.State nat unit :=
+  M.modify (fun s => s - i).
+
+Definition get10 : State nat nat:= return_ 10.
+
+Definition count15 : State nat unit :=
+ add_s 1;;
+ add_s 2;;
+ add_s 3;;
+ add_s 4;;
+ add_s 5;;
+ return_ tt.
+
+Notation "{{ P }} m {{ Q }}" := (hoareTripleS P m Q)
+  (at level 90, format "'[' '[' {{  P  }}  ']' '/  ' '[' m ']' '['  {{  Q  }} ']' ']'") : monad_scope.
+
+Lemma l_add_s :
+ forall (n i : nat), {{fun (s : nat) => s = n}} add_s i {{fun (_ : unit) (s : nat) => s = n + i}}.
+  Proof.
+  intros n i s H.
+  unfold add_s.
+  apply modify.
+  auto.
+  Qed.
+
+Lemma l_count15 : {{fun s : nat => s = init_S1}} count15 {{fun (_ : unit ) (s : nat) => s = 15}}.
+  Proof.
+  apply bindRev with (Q := (fun (_ : unit ) (s : nat) => s = 1)); try apply l_add_s.
+  + intros; apply bindRev with (Q := (fun (_ : unit ) (s : nat) => s = 3)) ; try apply l_add_s.
+  - intros; apply bindRev with (Q := (fun (_ : unit ) (s : nat) => s = 6)) ; try apply l_add_s.
+  * intros; apply bindRev with (Q := (fun (_ : unit ) (s : nat) => s = 10)) ; try apply l_add_s.
+    intros; apply bindRev with (Q := (fun (_ : unit ) (s : nat) => s = 15)) ; try apply l_add_s.
+    intros. intros S H. trivial.
+  Qed.
+
+Definition count42 : State nat unit
+ := for j = 0 to 3 {{ 
+    add_s j ;;
+    add_s j ;;
+    perf x <- get10;
+    add_s x ;;
+    add_s j ;;
+    add_s j
+  }} .
+
+Definition counti : State nat () :=
+   for i = 0 to 20 {{
+    (add_s i)
+  }}.
+
+Lemma l_counti : hoareTripleS (fun s : nat => s = init_S1) counti (fun (_ : unit ) (s : nat) => s = 42).
+  Proof.
+  eapply bindRev.
+  Admitted.
+
+Lemma l_count42 : hoareTripleS (fun s : nat => s = init_S1) count42 (fun (_ : unit ) (s : nat) => s = 42).
+  Proof.
+  eapply bindRev.
+  unfold count42.
+  unfold loopT_liftT.
+  eapply bindRev.
+  Admitted.
+
+Check count42.
+
+Compute runState (
+  count42
+  ) init_S1.
+
+Compute runState (
+  for i = 0 to 5 {{
+    add_s i 
+  }} ;; 
+  for j = 0 to 5 
+  {{ 
+    add_s j 
+  }} ) init_S1.
+
+Compute runState (
+  for i = 0 to 5 {{
+    add_s i 
+  }} ;; 
+  perf x <- get10 ;
+  add_s x ;;
+  for j = 0 to 5 
+  {{ 
+    add_s j 
+  }} ) init_S1.
+
+Open Scope list_scope.
+
+Definition nth2 := 4.
+
+Definition init_S2 : list nat := [].
+
+Definition addElement (val : nat) : State (list nat) unit :=
+  M.modify (fun s => val :: s).
+
+Compute runState (for i = 0 to nth2 {{ for j = 0 to nth2 {{addElement (i+j) }} }} ) init_S2.
+
+(* exit *)
+
+Definition test_exit : State nat () :=
+   for_e i = 0 to 20 {{
+    if (i =? 5) then exit
+    else (loopT_liftT (add_s i))
+  }}.
+
+
+Lemma l_test_exit : hoareTripleS (fun s : nat => s = 0) test_exit (fun (_ : unit ) (s : nat) => s = 0).
+  Proof.
+  eapply bindRev.
+  Admitted.
+
+Open Scope Z_scope.
+
+(* if/else *)
+
+Definition add_z (i : nat) : M.State Z unit :=
+  M.modify (fun s => s + Z.of_nat i).
+
+Definition minus_z (i : nat) : M.State Z unit :=
+  M.modify (fun s => s - Z.of_nat i).
+
+Definition init_Z1 : Z := 0.
+
+Compute runState (
+  for i = 0 to 6 {{
+    if (Z.eqb (Z.modulo (Z.of_nat i) 2) 0) then
+      add_z i 
+    else 
+      minus_z i
+  }}
+  ) init_Z1.
+
+End Test.
