demo/Test.v
@@ -1,0 +1,453 @@
+(* Require Import Program ZArith.
+
+Set Implicit Arguments.
+
+Import Notations.
+
+Local Notation "f ∘ g" := (fun x => f (g x)) (at level 40, left associativity).
+
+(* State Monad *)
+
+Record S : Type:= {
+  r : nat
+}.
+
+Definition State (A : Type) := S -> A * S.
+
+(* Arguments State [ A ]. *)
+
+(* forall {A}, A -> m A; *)
+Definition state_pure A (a : A) : State A := 
+  fun s => (a,s).
+
+(* state_bind = 
+fun (A : Type) (st_a : State A) (B : Type) (f : A -> State B) (s : S) => let (a, s0) := st_a s in f a s0
+     : forall A : Type, State A -> forall B : Type, (A -> State B) -> S -> B * S *)
+Definition state_bind {A B} (st_a : State A) (f : A -> State B)  : State B :=
+  fun s => let (a, s0) := st_a s in f a s0.
+
+
+(*    bind: forall {A}, m A -> forall {B}, (A -> m B) -> m B;
+  bind_right_unit: forall A (a: m A), a = bind a return_;
+  bind_left_unit: forall A (a: A) B (f: A -> m B),
+             f a = bind (return_ a) f;
+  bind_associativity: forall A (ma: m A) B f C (g: B -> m C),
+                 bind ma (fun  x=> bind (f x) g) = bind (bind ma f) g *)
+(* Lemma bind_right_unit *)
+
+Lemma state_bind_right_unit : 
+  forall (A : Type) (a: State A), a = state_bind a (@ state_pure A).
+  Proof.
+  intros.
+  unfold state_bind.
+  apply functional_extensionality.
+  intros.
+  destruct (a x).
+  reflexivity.
+  Qed.
+
+Lemma state_bind_left_unit :
+   forall A (a: A) B (f: A -> State B),
+             f a = state_bind (state_pure a) f.
+   Proof.
+   auto.
+   Qed.
+
+Lemma state_bind_associativity :
+  forall A (ma: State A) B f C (g: B -> State C),
+                 state_bind ma (fun x => state_bind (f x) g) = state_bind (state_bind ma f) g.
+  Proof.
+  intros.
+  unfold state_bind.
+  apply functional_extensionality.
+  intros.
+  destruct (ma x).
+  reflexivity.
+  Qed.
+
+Definition put (x : S) : State () :=
+  fun _ => (tt,x).
+
+Definition get : State S :=
+  fun x => (x,x).
+
+Definition runState  {A} (op : State A) : S -> A * S := op.
+Definition evalState {A} (op : State A) : S -> A := fst ∘ op.
+Definition execState {A} (op : State A) : S -> S := snd ∘ op.
+
+Notation "m1 ;; m2" := (state_bind m1 (fun _ => m2))  (at level 60, right associativity) : monad_scope.
+Notation "'perf' x '<-' m ';' e" := (state_bind m (fun x => e))
+  (at level 60, x ident, m at level 200, e at level 60) : monad_scope.
+
+Open Scope monad_scope.
+
+(* modify = 
+fun (S : Type) (f : S -> S) => perf s <- getS (S:=S); putS (f s)
+     : forall S : Type, (S -> S) -> State S () *)
+Definition modify (f : S -> S) : State () :=
+  perf s <- get; put (f s).
+
+Definition Assertion := S -> Prop.
+
+Definition hoareTripleS {A} (P : S -> Prop) (m : State A) (Q : A -> S -> Prop) : Prop :=
+  forall (s : S), P s -> let (a, s') := m s in Q a s'.
+
+Notation "{{ P }} m {{ Q }}" := (hoareTripleS P m Q)
+  (at level 90, format "'[' '[' {{  P  }}  ']' '/  ' '[' m ']' '['  {{  Q  }} ']' ']'") : monad_scope.
+
+Lemma ret  (A : Type) (a : A) (P : A -> Assertion) : {{ P a }} state_pure a {{ P }}.
+Proof.
+intros s H; trivial.
+Qed.
+
+(* Triplet de hoare sur la séquence *)
+Lemma bind  (A B : Type) (m : State A) (f : A -> State B) (P : Assertion)( Q : A -> Assertion) (R : B -> Assertion) :
+  (forall a, {{ Q a }} f a {{ R }}) -> {{ P }} m {{ Q }} -> {{ P }} perf x <- m ; f x {{ R }}.
+Proof. 
+intros H1 H2 s H3.
+unfold state_bind.
+case_eq (m s).
+intros.
+apply H2 in H3.
+case_eq (f a s0).
+intros b s'' H5.
+Admitted.
+
+Definition wp {A : Type} (P : A -> S -> Prop) (m : State A) :=
+  fun s => let (a,s') := m s in P a s'.
+
+Lemma wpIsPrecondition {A : Type} (P : A -> S -> Prop) (m : State A) :
+  {{ wp P m }} m {{ P }}.
+  Proof.
+  unfold wp.
+  congruence.
+  Qed.
+
+Lemma wpIsWeakestPrecondition
+  (A : Type) (P : A -> S -> Prop) (Q : S -> Prop) (m : State A) :
+  {{ Q }} m {{ P }} -> forall s, Q s -> (wp P m) s.
+  Proof.
+  trivial.
+  Qed.
+
+Lemma assoc (A B C : Type)(m : State A)(f : A -> State B)(g : B -> State C) :
+  perf y <-
+    perf x <- m ;
+    f x ;
+  g y =
+  perf x <- m ;
+  perf y <- f x ;
+  g y.
+  Proof.
+  extensionality s; unfold state_bind; case (m s); trivial; tauto.
+  Qed.
+
+Lemma l_put (s : S) (P : unit -> Assertion) : {{ fun _ => P tt s }} put s {{ P }}.
+Proof.
+intros s0 H;trivial.
+Qed.
+
+Lemma l_get (P : S -> Assertion) : {{ fun s => P s s }} get {{ P }}.
+Proof.
+intros s H; trivial.
+Qed.
+
+Lemma bindRev (A B : Type) (m : State A) (f : A -> State B) (P : Assertion)( Q : A -> Assertion) (R : B -> Assertion) :
+  {{ P }} m {{ Q }} -> (forall a, {{ Q a }} f a {{ R }}) -> {{ P }} perf x <- m ; f x {{ R }}.
+Proof.
+intros; eapply bind ; eassumption.
+Qed.
+
+Lemma weaken (A : Type) (m : State A) (P Q : Assertion) (R : A -> Assertion) :
+  {{ Q }} m {{ R }} -> (forall s, P s -> Q s) -> {{ P }} m {{ R }}.
+Proof.
+intros H1 H2 s H3.
+apply H2 in H3. 
+apply H1 in H3.
+assumption. 
+Qed.
+
+Lemma strengthen (A : Type) (m : State A) (P: Assertion) (Q R: A -> Assertion) :
+  {{ P }} m {{ R }} -> (forall s a, R a s -> Q a s) -> {{ P }} m {{ Q }}.
+Proof.
+intros H1 H2 s H3.
+apply H1 in H3.
+Admitted.
+
+
+Lemma l_modify f (P : () -> Assertion) : {{ fun s => P tt (f s) }} modify f {{ P }}.
+Proof.
+unfold modify.
+eapply bind.
+intros.
+eapply l_put.
+simpl.
+eapply weaken.
+eapply l_get.
+intros. simpl.
+assumption.
+Qed.
+
+(* End state_monad.
+
+Section loop_monad. *)
+
+Definition LoopT a : Type := (forall (r : Type), (a -> State r) -> State r).
+
+Definition runLoopT {a r} (loop : LoopT a) (next : a -> State r) :  State r :=
+  loop r next.
+(* next : (a -> LoopT r) *)
+
+(* Arguments runLoopT {_} {_} {_} {_}. *)
+
+Definition loopT_pure {A} (a : A) : LoopT A :=
+  fun _ next => next a.
+
+(* >>= for Loop *)
+Definition loopT_bind {A} (x : LoopT A) {B} (k : A -> LoopT B) : LoopT B :=
+  (fun _ next =>
+    let f' := (fun a => runLoopT (k a) next) in
+    runLoopT x f').
+
+(*   bind_right_unit: forall A (a: m A), a = bind a return_;
+  bind_left_unit: forall A (a: A) B (f: A -> m B),
+             f a = bind (return_ a) f;
+  bind_associativity: forall A (ma: m A) B f C (g: B -> m C),
+                 bind ma (fun  x=> bind (f x) g) = bind (bind ma f) g *)
+Lemma loopT_bind_right_unit :
+  forall A (a : LoopT A), a = loopT_bind a loopT_pure.
+  Proof.
+  auto.
+  Qed.
+
+Lemma loopT_bind_left_unit :
+  forall A (a: A) B (f: A -> LoopT B),
+             f a = loopT_bind (loopT_pure a) f.
+  Proof.
+  auto.
+  Qed.
+
+Lemma loopT_bind_associativity :
+  forall A (ma: LoopT A) B f C (g: B -> LoopT C),
+                 loopT_bind ma (fun  x=> loopT_bind (f x) g) = loopT_bind (loopT_bind ma f) g.
+  Proof.
+  auto.
+  Qed.
+
+(* forall {A}, m A -> t m A; *)
+Definition loopT_liftT {A} (m : State A) : LoopT A :=
+(fun _ cont => state_bind m cont).
+
+(* Variable S : Type.
+
+Definition stepLoopT {e a}  (body : LoopT e (State S) a) (next : a -> (State S) e) : (State S) e :=
+  runLoopT body (return_) next. *)
+
+Definition stepLoopT {a} (body : LoopT a) (next : a -> State ()) : State () :=
+  runLoopT body next.
+
+(* lifT_id : forall {A : Type} (a : A), (liftT ∘ return_) a = return_ a;
+lifT_bind : forall A B (ma : m A) (k : A -> m B), liftT (ma >>= k) = (liftT ma) >>= (liftT ∘ k); *)
+
+Lemma loopT_liftT_id :
+  forall {A : Type} (a : A), (loopT_liftT ∘ (@ state_pure A)) a = loopT_pure a.
+  Proof.
+  intros;cbn.
+  unfold loopT_liftT.
+  unfold loopT_pure.
+  extensionality r.
+  extensionality exit.
+  extensionality cont.
+  rewrite <- state_bind_left_unit.
+  reflexivity.
+  Qed.
+
+Lemma loopT_lifT_bind :
+  forall A B (ma : State A) (k : A -> State B), 
+      loopT_liftT (state_bind ma k) = loopT_bind (loopT_liftT ma) (loopT_liftT ∘ k).
+  Proof.
+  intros;cbn.
+  unfold loopT_liftT.
+  unfold loopT_bind.
+  unfold runLoopT.
+  extensionality r.
+  extensionality exit.
+  extensionality cont.
+  rewrite state_bind_associativity.
+  reflexivity.
+  Qed.
+
+Import List.
+
+Definition foreach''{v} (values : list v) {a} (body : v -> LoopT a) : State () :=
+  fold_right
+    (fun x next => stepLoopT (body x) (fun _ => next))
+    (state_pure tt)
+    values.
+
+Definition foreach'(min max : nat) (body : nat -> LoopT ()) : State () :=
+  foreach'' (seq min (max-min)) body.
+
+Notation "'for' i '=' min 'to' max '{{' body }}" := (foreach' min max (fun i => (loopT_liftT body))) (at level 60, i ident, min at level 60,
+max at level 60, body at level 60, right associativity) : monad_scope.
+
+Notation "'for2' i '=' min 'to' max '{{' body }}" := (foreach' min max (fun i => (body))) (at level 60, i ident, min at level 60,
+max at level 60, body at level 60, right associativity) : monad_scope.
+
+(* Au dessus de ma fonction foreach *)
+
+Definition hoareTripleL {A B} (P : Assertion) (m : LoopT A) (Q : B -> Assertion) : Prop := 
+  forall (s : S) (next : A -> State B), P s -> let (b, s') := (runLoopT m next) s in Q b s'.
+
+Notation "{[ P ]} m {[ Q ]}" := (hoareTripleL P m Q)
+  (at level 90, format "'[' '[' {[  P  ]}  ']' '/  ' '[' m ']' '['  {[  Q  ]} ']' ']'") : monad_scope.
+
+(* Lie une monade d'état à sa monade loop associée *)
+(* Definition match_monad {A} : LoopT A -> State A -> Prop :=
+  forall (mL : LoopT A) (mS : State A), loopT_liftT mS = mL. *)
+
+(* Lemma match_monad_spec {A} (mL : LoopT A) (mS : State A): 
+  loopT_liftT mS = mL -> match_monad mL mS.
+  Proof.
+  constructor.
+  assumption.
+  Qed. *)
+
+(* Inductive foreach_L {A B} (P : Assertion) (m : LoopT A) (Q : B -> Assertion) : Prop :=
+  | For_E :
+  | For_N : forall A', HoareTriple_L P m Q ->  foreach_L P m Q -> foreach_L *)
+
+(* Lemma bind  (A B : Type) (m : State A) (f : A -> State B) (P : Assertion)
+( Q : A -> Assertion) (R : B -> Assertion) :
+  (forall a, {{ Q a }} f a {{ R }}) -> {{ P }} m {{ Q }} -> {{ P }} 
+  perf x <- m ; f x {{ R }}.
+ *)
+Lemma loopT_to_state (P : S -> Prop) (Q : () -> S -> Prop) (mo : State ()) :
+  (forall mT : LoopT (), mT = loopT_liftT mo -> {{P}} mo {{Q}} -> 
+  {[P]} mT {[Q]}).
+  Proof.
+  intros.
+  rewrite H.
+  unfold loopT_liftT.
+  
+  unfold state_bind.
+  intros s next Hp.
+  unfold hoareTripleS in H0.
+  intros.
+  simpl.
+  case_eq (m', s).
+  intros.
+  apply H0.
+  unfold runLoopT.
+  destruct (mo s).
+  case (next u s0).
+  intros.
+  
+  Admitted.
+
+Lemma foreach_rule (min max : nat) (P : S -> Prop) (body : nat -> LoopT ())
+  : (forall (it:nat), {[fun s => P s /\ (Nat.le min it) /\ (it < max)]} 
+  body it {[fun (_: unit) => P]}) -> 
+  {{P}} foreach' min max (body) {{fun _ => P}} .
+  Admitted.
+
+(* Lemma state_to_loop (P : S -> Prop) (body : nat -> State ()) : 
+  forall (it:nat), {{fun s => P s /\ (min <= it) /\ (it < max)}} 
+  body it {[fun (_: unit) => P]} -> 	  body it {[fun (_: unit) => P]}) -> 
+  {{P}} foreach' min max (body) {{fun _ => P}} . *)
+
+(* Lemma foreach_rule (min max : nat) (P : S -> Prop) (m : nat -> State ())
+  : (forall (it:nat), {{fun s => P s /\ (min <= it < max)}} m it {{fun _ => P}}
+    -> {{P}}foreach' min max (fun it0 => loopT_liftT (m it0)) {{fun _ => P}}).
+  Proof.
+  intros it.
+  Admitted. *)
+
+Definition init_state : S := {|r := 1|}.
+
+Definition add_s (i : nat) : State unit :=
+  modify (fun s => {| r := s.(r) + i |}).
+
+Definition min_s (i : nat) : State unit :=
+modify (fun s => {| r := s.(r) - i |}).
+
+Definition mul_s (i : nat) : State unit :=
+  modify (fun s => {| r := s.(r) * i |}).
+
+Definition fac5 : State unit :=
+  for i = 1 to 6 {{
+    mul_s i
+  }}.
+
+Compute runState fac5 init_state.
+
+Definition slow_add (m : nat) : State unit :=
+  for i = 0 to m {{
+    add_s 1
+  }}.
+
+Definition slow_add2 (m : nat) : State unit :=
+  for i = 0 to m {{
+    if ((Nat.modulo i 2) =? 0) then
+      add_s 1
+    else
+      add_s 2
+  }}.
+
+Compute runState (slow_add 7) init_state.
+
+(* Lemma l_slow_add (n m : nat): 
+ {{(fun s : S => r s = n)}} slow_add m {{(fun (_ : unit ) (s : S) => r s = (Nat.add m n))}}.
+Proof.
+eapply strengthen.
+eapply weaken.
+unfold slow_add.
+eapply foreach_rule.
+2 : { intros.
+      assert (H2 : r s <= (n + m)).
+      - 
+      apply Nat.eq_le_incl in H.
+      eapply le_plus_trans.
+      trivial.
+      - apply H2. }
++ intros. eapply loopT_to_state with (add_s 1).
+  - trivial.
+  - admit. 
++ cbn.
+unfold add_s.
+eapply weaken.
+apply l_modify.
+intros.
+simpl.
+trivial.
+  - intros.
+    simpl in H.
+    
+Admitted. *)
+
+Compute runState fac5 init_state.
+
+Lemma l_fac5 : 
+ {{(fun s : S => r s = 1)}} fac5 {{(fun (_ : unit ) (s : S) => r s = 120)}}.
+Proof.
+eapply strengthen.
+unfold fac5.
+eapply foreach_rule.
++ intros.
+  
+  - eapply weaken.
+unfold l.
+intros s H.
+eapply foreach_rule.
+
++ admit.
++ admit.
+
+(* Lemma l_add_s :
+ forall (n i : nat), {{fun (s : S) => val s = n}} add_s i {{fun (_ : unit) (s : S) => val s = (n + i)}}.
+  Proof.
+  intros n i s H.
+  unfold add_s.
+  apply l_modify.
+  auto.
+  Qed. *) *)
