demo/TestLoop.v
@@ -1,0 +1,411 @@
+Require Import LoopV2 Program List ZArith Arith Coq.Logic.Classical_Prop.
+
+Set Implicit Arguments.
+
+Section ResTab.
+
+(* Axiom tableSize : nat.
+Axiom maxTimeOut : nat. *)
+Axiom defaultValue : nat.
+
+(* Axiom tableSizeNotZero : tableSize > 0.
+Axiom timeOutNotZero : maxTimeOut > 0.
+Axiom timeOutBiggerTableSize : tableSize < maxTimeOut. *)
+
+Definition tab : Type := list nat.
+
+Definition addElement (n : nat) : State tab unit :=
+  modify (fun s => n :: s).
+
+Lemma LaddElement (n : nat) (P : unit -> tab -> Prop) :
+{{fun  s => P tt (n :: s) }} addElement n {{P}}.
+Proof.
+unfold addElement.
+eapply weaken.
+eapply l_modify.
+intros.
+simpl.
+assumption.
+Qed.
+
+
+Definition readTabEntry (idx : nat) (ltab : tab) : nat :=
+  nth idx ltab defaultValue.
+
+
+Fixpoint changeElement (i n : nat) (l: tab) : tab :=
+ match (l,i) with
+  | ([], _) => []
+  | (a :: l', 0) => n :: l'
+  | (a :: l', S i') => a :: changeElement i' n l'
+  end.
+
+SearchAbout nil.
+
+Lemma LchangeElement_size1 (l : tab)  :
+  forall (i n : nat), length l = length (changeElement i n l).
+  Admitted.
+
+Lemma LchangeElement_size2 (l : tab)  :
+  forall (i n : nat), length (changeElement i n l) = length l.
+  Admitted.
+
+Lemma LchangeElement_in (i : nat) (n : nat) :
+  forall (l : tab)  , i < length l -> In n (changeElement i n l).
+  Proof.
+  intro l.
+  generalize i.
+  induction l.
+  - intros.
+    simpl in H.
+    omega.
+  - simpl in *.
+    induction i0.
+    + intros. simpl. auto.
+    + intros.
+      apply lt_S_n in H.
+      simpl.
+      right.
+      apply IHl.
+      apply H.
+  Qed.
+
+Lemma LchangeElement_nth (i : nat) (n : nat) :
+  forall (l : tab)  , i < length l -> readTabEntry i (changeElement i n l) = n.
+  Proof.
+(*   Admitted. *)
+  intro l.
+  generalize i.
+  induction l.
+  - intros.
+    simpl in H.
+    omega.
+  - simpl in *.
+    induction i0.
+    + intros. simpl. auto.
+    + intros.
+      apply lt_S_n in H.
+      simpl.
+      apply IHl.
+      apply H.
+  Qed.
+
+Lemma LchangeElement_inf (i : nat) (n : nat) :
+  forall (l : tab) (j : nat) , j <= i < length l -> readTabEntry j (changeElement i n l) = readTabEntry j l.
+  Admitted.
+
+Definition changeTab (i n: nat) : State tab unit :=
+  modify (fun s => changeElement i n s).
+
+Lemma LchangeTab (i : nat) (n : nat) (P : unit -> tab -> Prop) :
+  {{fun  s => P tt (changeElement i n s) }} changeTab i n {{P}}.
+  Proof.
+  unfold addElement.
+  eapply weaken.
+  eapply l_modify.
+  intros.
+  simpl.
+  assumption.
+  Qed.
+
+Definition init_table (size : nat) : State tab unit :=
+  for i = size to 0 {{
+    addElement (i)
+  }}.
+
+Definition init_tablei (size : nat) : State tab unit :=
+  for i = size to 0 {{
+    changeTab (i - 1) i
+  }}.
+
+Definition init_tablei2 (size : nat) : State tab unit :=
+  for2 i = 0 to size {{
+    changeTab i (i + 1)
+  }}.
+
+Definition init_tableT (size : nat) : State tab unit :=
+  foreachT size 0 (fun i => loopT_liftT (changeTab i (i + 1))).
+
+Compute runState (init_tablei2 10) [0;0;0;0;0;0;0;0;0;0].
+
+Compute runState (init_tableT 10) [0;0;0;0;0;0;0;0;0;0].
+
+Definition init_table0 (size : nat) : State tab unit :=
+  for i = size to 0 {{
+    addElement 0
+  }}.
+
+Definition initPgoodi (curidx : nat) (l : tab) : Prop :=
+  forall i : nat, curidx < i < length l -> readTabEntry i l = i+1.
+
+Definition initPgoodi_inv (curidx : nat) (l : tab) : Prop :=
+  forall i : nat, i <= curidx < length l -> readTabEntry i l = i+1.
+
+(* Definition init_table2 (size : nat) : State tab unit :=
+  for_e i = maxTimeOut to 0 {{$
+    if (
+    addElement (size - i + 1)
+  }}. *)
+
+Definition initPgoodEnd0 (l : tab) : Prop :=
+  forall i : nat, i < length l -> readTabEntry i l = 0.
+
+Definition initPgoodEndI (l : tab) : Prop :=
+  forall i : nat, i < length l -> readTabEntry i l = i + 1.
+
+Compute runState (init_tablei 10) [0;0;0;0;0;0;0;0;0;0].
+
+Lemma initPEntry (size : nat)  :
+  {{fun (s : tab) => initPgoodi size s /\ (length s > size)}} init_tablei size 
+  {{fun _ (s : tab) => initPgoodEndI s}}.
+  Proof.
+  unfold init_tablei.
+  apply strengthen with (fun _ (s : tab) => initPgoodi size s /\ length s > size).
+  induction size.
+  + cbn.
+    intros s H; trivial.
+  + unfold foreach.
+    cbn.
+    eapply bindRev.
+    - unfold runLoopT.
+      unfold loopT_liftT.
+      unfold state_liftM.
+      eapply bindRev.
+      eapply weaken.
+      eapply LchangeTab.
+      cbn.
+      intros.
+      pattern s in H.
+       match type of H with
+      | ?HT s => instantiate (1 := fun tt s => HT s )
+      end.
+      simpl.
+      destruct H as (Hinit & Hlen).
+(*       
+    unfold initPgoodi in H.
+    intuition.
+    cbn.
+    eapply *)
+  Admitted.  
+ 
+Definition Prop1 (n : nat) (st : tab) : Prop :=
+  (length st = n) /\ initPgoodi n st.
+
+Definition Prop2 (n : nat) (st : tab) : Prop :=
+  (length st > n) /\ initPgoodi_inv n st.
+
+Lemma initPEntryI2 (size : nat) :
+  {{fun (s : tab) => Prop2 0 s }} init_tablei2 size 
+  {{fun _ (s : tab) => initPgoodEndI s}}.
+  Proof.
+  unfold init_tablei.
+  eapply strengthen.
+  eapply foreach2_rule2; unfold Prop2 in *.
+  + intros.
+    unfold Prop2.
+    eapply weaken.
+    eapply l_modify.
+    intros.
+    destruct H.
+    destruct H.
+    unfold initPgoodi_inv in *.
+    split.
+    intuition.
+    assert (length (changeElement it (it + 1) s) = length s).
+(*     rewrite <- H at 3. *)
+    apply LchangeElement_size2.
+    omega.
+    intros.
+    pose proof LchangeElement_nth.
+    intuition.
+    assert (i < length (changeElement it (it + 1) s)) by omega.
+    generalize (H3 it (it + 1) s).
+    intros.
+    assert (readTabEntry it (changeElement it (it + 1) s) = it + 1).
+    apply H7.
+    omega.
+    pose proof LchangeElement_inf.
+    generalize (H9 it (it + 1) s i).
+    intros.
+    assert (readTabEntry i s = i + 1).
+    auto.
+    rewrite <- H11.
+    apply H10.
+    omega.
+  + unfold Prop2.
+    intros s [] HP.
+    destruct HP.
+(*     unfold initPgoodEndI. *)
+    (* intros. *)
+    unfold initPgoodi_inv in H0.
+    unfold initPgoodEndI.
+    Admitted.
+(*     replace (i <= size < length s) with (i < length s) in H0.
+    intros.
+    apply H0.
+    split.
+    
+ Qed. *)
+
+Definition getSize : State tab nat :=
+  perf s <- (@get tab);
+  state_pure (length s).
+
+Definition init_tablei3 : State tab unit :=
+  perf size <- getSize ;
+  for2 i = 0 to size {{
+    changeTab i (i + 1)
+  }}.
+
+Definition Prop3 (n : nat) (st : tab) : Prop :=
+  initPgoodi_inv n st.
+
+Lemma LgetSizeWp (P : nat -> tab -> Prop) :
+{{wp P getSize}} getSize {{P}}.
+  Proof.
+  eapply wpIsPrecondition.
+  Qed.
+
+Lemma LgetSize P : 
+{{ fun s => P s }} getSize 
+{{ fun size s => P s /\ size = length s }}.
+  Proof.
+    eapply weaken.
+    eapply LgetSizeWp.
+    cbn.
+    intros.
+    intuition.
+  Qed.
+
+(* Lemma LgetSize (P : nat -> tab -> Prop) :
+{{ fun s : tab => P (length s)  s }} 
+  getSize {{ fun s => P s}}.
+  Proof.
+  unfold getSize.
+  eapply bindRev.
+  + apply l_get. *)
+
+Lemma initPEntryI3 :
+  {{fun (s : tab) => Prop2 0 s }} init_tablei3 
+  {{fun _ (s : tab) => initPgoodEndI s}}.
+  Proof.
+  unfold init_tablei3.
+  eapply bindRev.
+  + apply LgetSize.
+  + intros.
+  eapply strengthen.
+  eapply foreach2_rule3. unfold Prop2 in *.
+  - intros.
+    eapply weaken.
+    eapply l_modify.
+    intros.
+    destruct H.
+    unfold initPgoodi_inv in *.
+    intuition.
+    assert (length (changeElement it (it + 1) s) = length s).
+    apply LchangeElement_size2.
+    omega. (* 
+    intros. *)
+    pose proof LchangeElement_nth.
+(*     intuition. *)
+    assert (i < length (changeElement it (it + 1) s)) by omega.
+    generalize (H3 it (it + 1) s).
+    intros.
+    assert (readTabEntry it (changeElement it (it + 1) s) = it + 1).
+    apply H8.
+    omega.
+    pose proof LchangeElement_inf.
+    generalize (H10 it (it + 1) s i).
+    intros.
+    assert (readTabEntry i s = i + 1).
+    auto.
+    rewrite <- H12.
+    apply H10.
+    omega.
+    assert (length (changeElement it (it + 1) s) = length s).
+    apply LchangeElement_size2.
+    omega.
+  - simpl.
+    intros s [] H.
+    destruct H.
+    unfold Prop2 in *.
+    destruct H.
+    unfold initPgoodi_inv .
+    omega.
+Qed.
+
+(* Lemma initPEntryI (size : nat)  :
+  {{fun (s : tab) => Prop1 size s }} init_tablei size 
+  {{fun _ (s : tab) => initPgoodEndI s}}.
+  Proof.
+  unfold init_table0.
+  eapply strengthen.
+  eapply foreach_rule2; unfold Prop1.
+  + intros.
+    unfold changeTab.
+    eapply weaken.
+    eapply l_modify.
+    intros.
+    destruct H.
+    simpl.
+    split.
+    intuition.
+    rewrite <- H1 at 3.
+    apply LchangeElement_size2.
+    unfold initPgoodi in *.
+    intros.
+    unfold readTabEntry in *.
+    destruct H.
+    SearchAbout nth.
+    pose proof LchangeElement_nth.
+    generalize (H3 (it - 1) (it)).
+    intros.
+    apply H2.
+    apply nth_in_or_default
+    generalize (H (i + 1)).
+    intros.
+    assert (i + 1 > size).
+    omega.
+    apply H4 in H5.
+    SearchAbout nth.
+    pose proof app_nth2.
+    generalize (H6 nat [0] s 2 (i+2)).
+    intros.
+    assert ( i + 2 >= length [0] ).
+    cbn.
+    omega.
+    apply H7 in H8.
+    rewrite <- H5 at 2.
+    cbn.
+    case_eq i.
+    intros.
+    omega.
+    intros.
+    subst.
+    simpl in H8.
+    simpl in H7.
+    replace (i + 1 - 1) with i in * by omega.
+    case_eq (i + 1).
+    intros.
+    omega.
+    intros.
+    rewrite H9 in H8.
+    cbn.
+    cbn in H7.
+    pattern s in H.
+     match type of H with
+    | ?HT s => instantiate (1 := fun tt s => HT s /\ 
+                 readTabEntry 0 s = (size - it + 1 ) )
+    end.
+    simpl.
+    split.
+    assumption.
+    unfold readTabEntry.
+    cbn.
+    omega.
+    cbn.
+    intros.
+    trivial.
+  Qed. *)
+
+End ResTab.
